LRrule/extract.v
@@ -14,7 +14,8 @@
 (******************************************************************************)
 Require Import ssreflect ssrbool ssrfun ssrnat eqtype finfun fintype choice seq tuple.
 Require Import finset perm.
-Require Import subseq partition ordtype schensted congr plactic green greeninv std.
+Require Import subseq partition ordtype schensted congr plactic green greeninv
+        std stdtab.
 
 Require Import Wf_nat.
 Extraction Inline Wf_nat.lt_wf_rec1 Wf_nat.lt_wf_rec
@@ -44,10 +45,13 @@ Extract Constant beq_nat => "( = )".
 
 Let RSbijnat := (@RSbij nat_ordType).
 Let RSbijinvnat := (@RSbijinv nat_ordType).
+Let RStabnat := (@RStab nat_ordType).
+Let RStabinvnat := (@RStabinv nat_ordType).
 
 Extraction "extract/schensted.ml"
            RS RSbijnat RSbijinvnat
            plactcongr
            greenRow greenCol
            is_std std.std
+           RStabnat RStabinvnat
 .
